weak prp prf refactor

theories/paris/examples/prp_prf_weak.v
@@ -1,85 +1,43 @@
 From clutch.paris Require Export paris map list prf prp.
 Set Default Proof Using "Type*".
 
-Section prf_prp.
+Section prp_prf.
 
-  (* This is the same as the simple hash *)
+  (* The weak PRP/PRF Switching Lemma.
+
+     We prove that (up to error) the idealized PRP and PRF are
+     indistinguishable in Q queries by calling each function Q times and
+     showing that both produce the same list of results.
+
+   *)
 
   Context `{!parisGS Σ}.
 
   Variable val_size : nat.
 
-  (*
-  Definition coll_free (m : gmap nat Z) :=
-    forall k1 k2,
-      is_Some (m !! k1) ->
-      is_Some (m !! k2) ->
-      m !!! k1 = m !!! k2 ->
-      k1 = k2.
-
-  Lemma coll_free_insert (m : gmap nat Z) (n : nat) (z : Z) :
-    m !! n = None ->
-    coll_free m ->
-    Forall (λ x, z ≠ snd x) (gmap_to_list m) ->
-    coll_free (<[ n := z ]>m).
-  Proof.
-    intros Hnone Hcoll HForall.
-    intros k1 k2 Hk1 Hk2 Heq.
-    apply lookup_insert_is_Some' in Hk1.
-    apply lookup_insert_is_Some' in Hk2.
-    destruct (decide (n = k1)).
-    - destruct (decide (n = k2)); simplify_eq; auto.
-      destruct Hk2 as [|Hk2]; auto.
-      rewrite lookup_total_insert in Heq.
-      rewrite lookup_total_insert_ne // in Heq.
-      apply lookup_lookup_total in Hk2.
-      rewrite -Heq in Hk2.
-      eapply (Forall_iff (uncurry ((λ (k : nat) (v : Z), z ≠ v)))) in HForall; last first.
-      { intros (?&?); eauto. }
-      eapply map_Forall_to_list in HForall.
-      rewrite /map_Forall in HForall.
-      eapply HForall in Hk2; congruence.
-    - destruct (decide (n = k2)); simplify_eq; auto.
-      {
-        destruct Hk1 as [|Hk1]; auto.
-        rewrite lookup_total_insert in Heq.
-        rewrite lookup_total_insert_ne // in Heq.
-        apply lookup_lookup_total in Hk1.
-        rewrite Heq in Hk1.
-        eapply (Forall_iff (uncurry ((λ (k : nat) (v : Z), z ≠ v)))) in HForall; last first.
-        { intros (?&?); eauto. }
-        eapply map_Forall_to_list in HForall.
-        rewrite /map_Forall in HForall.
-        eapply HForall in Hk1; congruence.
-      }
-      rewrite ?lookup_total_insert_ne // in Heq.
-      destruct Hk1 as [|Hk1]; try congruence; [].
-      destruct Hk2 as [|Hk2]; try congruence; [].
-      apply Hcoll; eauto.
-  Qed.
-*)
-
   Definition is_sprp := is_sprp val_size.
   Definition random_permutation := random_permutation val_size.
   Definition is_random_function := is_random_function val_size.
   Definition random_function := random_function val_size.
+  Definition wPRP := wPRP val_size.
+  Definition wPRF := wPRF val_size val_size.
 
- Lemma wp_prf_prp_couple_eq_Some E K (k:Z) (f : val) (m : gmap nat Z) (sf : val) (sr : list Z) (n : nat) :
-   m !! n = Some k →
-   n <= val_size ->
-   {{{ ⤇ fill K (sf #n) ∗ is_random_function f m ∗ is_sprp sf m sr}}}
-     f #n @ E
-     {{{ RET #k;
-         ⤇ fill K (of_val #k) ∗ is_random_function f m ∗ is_sprp sf m sr }}}.
- Proof.
-   iIntros (Hsome Hrange Φ) "(HK&Hf&Hg) HΦ".
-   iMod (spec_prp_prev with "[$]") as "[HK Hg]"; [done|].
-   wp_apply (wp_random_function_prev with "[$]"); first done.
-   iIntros "Hf".
-   iApply "HΦ"; iFrame.
- Qed.
+  Lemma wp_prf_prp_couple_eq_Some E K (k:Z) (f : val) (m : gmap nat Z) (sf : val) (sr : list Z) (n : nat) :
+    m !! n = Some k →
+    n <= val_size ->
+    {{{ ⤇ fill K (sf #n) ∗ is_random_function f m ∗ is_sprp sf m sr}}}
+      f #n @ E
+      {{{ RET #k;
+          ⤇ fill K (of_val #k) ∗ is_random_function f m ∗ is_sprp sf m sr }}}.
+  Proof.
+    iIntros (Hsome Hrange Φ) "(HK&Hf&Hg) HΦ".
+    iMod (spec_prp_prev with "[$]") as "[HK Hg]"; [done|].
+    wp_apply (wp_random_function_prev with "[$]"); first done.
+    iIntros "Hf".
+    iApply "HΦ"; iFrame.
+  Qed.
 
- Lemma wp_prf_prp_couple_eq_err E K (f : val) (m : gmap nat Z) (sf : val) (sr : list Z) (n : nat) (ε : R):
+  Lemma wp_prf_prp_couple_eq_err E K (f : val) (m : gmap nat Z) (sf : val) (sr : list Z) (n : nat) (ε : R):
     m !! n = None →
     n <= val_size ->
     (∀ n' : nat, val_size < n' → m !! n' = None) ->
@@ -87,12 +45,12 @@ Section prf_prp.
     (((S val_size - (length sr)) / S val_size)%R <= ε)%R ->
     {{{ ⤇ fill K (sf #n) ∗ is_random_function f m ∗ is_sprp sf m sr ∗ ↯ ε }}}
       f #n @ E
-    {{{ (z: Z), RET #z;
-        ⤇ fill K (of_val #z) ∗ is_random_function f (<[ n := z ]>m) ∗
+      {{{ (z: Z), RET #z;
+          ⤇ fill K (of_val #z) ∗ is_random_function f (<[ n := z ]>m) ∗
           ∃ l1 l2,
-                ⌜ sr = l1 ++ z :: l2 ⌝ ∗
-          is_sprp sf (<[n := z]>m) (l1 ++ l2) }}}.
- Proof.
+            ⌜ sr = l1 ++ z :: l2 ⌝ ∗
+            is_sprp sf (<[n := z]>m) (l1 ++ l2) }}}.
+  Proof.
     iIntros (Hnone Hrange Hdom Hineq Hε Φ) "(HK & Hprf & Hprp & Herr) HΦ".
     iDestruct "Hprf" as (hm ->) "Hm".
     iDestruct "Hprp" as (lsm lsr) "(-> & Hsm & Hlsr & %Hperm)".
@@ -113,7 +71,6 @@ Section prf_prp.
     }
 
     edestruct (prp_None_non_full val_size) as (vl & Hvl); eauto.
-
 
     (* spec get *)
     tp_bind (get _ _).
@@ -136,10 +93,7 @@ Section prf_prp.
     tp_pure.
     tp_pure.
     tp_pure.
-    assert (#(S vl - 1) = #vl) as ->.
-    {
-     do 3 f_equal; lia.
-    }
+    assert (#(S vl - 1) = #vl) as ->. { do 3 f_equal; lia. }
 
     tp_bind (rand _)%E.
     iDestruct (ec_weaken with "[$]") as "Hε".
@@ -243,8 +197,6 @@ Section prf_prp.
     apply perm_skip.
     by rewrite Permutation_app_comm.
  Qed.
-
- Let dummy_scheme : val := ((λ: "_", #()),#()).
 
  Definition loop (f : val) (res : loc) :=
    (rec: "loop" "i" :=
@@ -416,15 +368,19 @@ Section prf_prp.
              ++ apply gset_semi_set.
   Qed.
 
+  (* We compare the "ideal" wPRP and wPRF games (as indicated by the #false
+     argument below); to ignore the "real" games (wPRP #true and wPRF #true),
+     we provide a dummy scheme. *)
+  Let dummy_scheme : val := ((λ: "_", #()),#()).
 
-  Lemma wp_wprf_wprp
+  Lemma wp_wPRF_wPRP
     E K (Q : nat) (ε : R) :
     ((fold_left Nat.add (seq 0 Q) 0%nat / S val_size)%R = ε) →
-    {{{ ↯ ε ∗ ⤇ fill K (wPRP val_size #false dummy_scheme #Q) }}}
-      wPRF val_size val_size #false dummy_scheme #Q @ E
+    {{{ ↯ ε ∗ ⤇ fill K (wPRP #false dummy_scheme #Q) }}}
+      wPRF #false dummy_scheme #Q @ E
       {{{ (vres : val), RET vres; ⤇ fill K vres }}}.
   Proof with (wp_pures ; tp_pures).
-    rewrite /wPRF/wPRP. iIntros (Hε) "%Φ (ε & spec) HΦ"...
+    rewrite /wPRF/wPRP/prf.wPRF/prp.wPRP. iIntros (Hε) "%Φ (ε & spec) HΦ"...
     tp_bind (prp.random_permutation _ #()).
     iMod (spec_random_permutation with "spec") as (rp) "(spec & rp)".
     wp_bind (random_function _).
@@ -466,208 +422,4 @@ Section prf_prp.
   Qed.
 
 
-Definition test_prf: val :=
-  λ: "n",
-    let: "f" := random_function #() in
-  letrec: "aux" "f" "i" :=
-    (if: "i" ≤ #0
-     then  "f"
-     else let: "x" := rand #val_size in
-          "f" "x";;
-          "aux" "f" ("i" - #1)) in
-      "aux" "f" "n".
-
-
-Definition test_prp: val :=
-  λ: "n",
-    let: "f" := random_permutation #() in
-    letrec: "aux" "f" "i" :=
-    (if: "i" ≤ #0
-     then  "f"
-     else let: "x" := rand #val_size in
-          "f" "x";;
-          "aux" "f" ("i" - #1)) in
-      "aux" "f" "n".
-
-
-
-Lemma wp_prf_prp_test_err_ind E K (f g:val) (m : gmap nat Z) (n k : nat) (l:list Z) (ε : R):
-  (0<=k<=n)%nat ->
-  ((S val_size) - (n-k))%nat <= length l ->
-  NoDup l ->
-  l⊆(Z.of_nat <$> seq 0 (S val_size)) ->
-  (forall x:Z, x∈ ((map_img m):gset _) -> x ∈ l -> False) ->
-  (dom m ⊆ set_seq 0 (S val_size))->
-  ((INR(fold_left (Nat.add) (seq (n-k) k) 0%nat) / INR (S val_size))%R <= ε)%R ->
-  {{{ ↯ ε ∗
-      is_random_function f m ∗
-      ⤇ fill K
-        ((rec: "aux" "f" "i" :=
-            if: "i" ≤ #0 then "f"
-            else let: "x" := rand #val_size in "f" "x";; "aux" "f" ("i" - #1))%V g #k) ∗
-      is_sprp g m l }}}
-    (rec: "aux" "f" "i" :=
-       if: "i" ≤ #0 then "f" else let: "x" := rand #val_size in "f" "x";; "aux" "f" ("i" - #1))%V f
-    #k
-    @ E
-    {{{ f, RET f;
-        ∃ g m l, ⤇ fill K (of_val g) ∗ is_random_function f m∗
-                 is_sprp g m l }}}.
-Proof.
-  iInduction k as [|k'] "IH" forall (m l ε).
-   - iIntros (Hn Hlen HNoDup Hsubseteq Hdom Hdom' Hε Φ) "(Hε & Hf & HK & Hg) HΦ".
-     tp_pures. wp_pures.
-     iModIntro.
-     iApply "HΦ".
-     iExists _,_,_. iFrame.
-
-   - iIntros (Hn Hlen HNoDup Hsubseteq Hdom Hdom' Hε Φ) "(Hε & Hf & HK & Hg) HΦ".
-     wp_pures.
-     wp_bind (rand _)%E.
-
-     tp_pures.
-     tp_bind (rand _)%E.
-     iMod (ec_zero) as "H0".
-     wp_apply (wp_couple_rand_rand_leq val_size val_size val_size val_size _ _ 0
-              with "[$]").
-     { done. }
-     { rewrite Rminus_diag /Rdiv Rmult_0_l /=//. }
-     iIntros (n2 m2) "[-> HK]".
-     iSimpl in "HK".
-     wp_pures.
-     wp_bind (f _).
-
-     tp_pures.
-     tp_bind (g _).
-     iAssert (↯ _ ∗ ↯ _)%I with "[Hε]" as "[Hε Hε']".
-     { iApply ec_split; last first.
-       - iApply ec_weaken; last done.
-         split; last first.
-         { etrans; last exact. rewrite <-cons_seq. rewrite fold_symmetric; [|lia|lia].
-           rewrite [foldr _ _ _]/=.
-           rewrite plus_INR Rdiv_plus_distr. done. }
-         apply Rplus_le_le_0_compat; apply Rcomplements.Rdiv_le_0_compat; real_solver.
-       - apply Rcomplements.Rdiv_le_0_compat; real_solver.
-       - apply Rcomplements.Rdiv_le_0_compat; real_solver. }
-     iAssert (⌜(n-S k')<S val_size⌝)%I with "[Hε]" as "%".
-     { pose proof Nat.lt_ge_cases (n-S k') (S val_size) as [|]; first done.
-       iExFalso. iApply ec_contradict; last done. simpl.
-       apply Rcomplements.Rle_div_r.
-       - pose proof pos_INR_S val_size. apply Rlt_gt. exact.
-       - rewrite Rmult_1_l. replace (_)%R with (INR (S val_size)); last by simpl. apply le_INR. lia. }
-     destruct (m!!fin_to_nat m2) eqn:Hm'.
-     + wp_apply (wp_prf_prp_couple_eq_Some with "[$]"); try done.
-       * apply elem_of_dom_2 in Hm'.
-         eapply elem_of_weaken in Hm'; last done.
-         rewrite elem_of_set_seq in Hm'. lia.
-       * iIntros "(HK & Hf & Hg)".
-         do 3 wp_pure. simpl.
-         do 3 tp_pure.
-         replace (Z.of_nat _ - 1)%Z with (Z.of_nat k')%Z; last lia.
-         iApply ("IH" with "[][][][][][][][$]"); try done.
-         -- iPureIntro. lia.
-         -- iPureIntro. lia.
-         -- simpl. iPureIntro. apply Req_le. rewrite fold_symmetric; try (intros; lia).
-            replace (S _)  with (n-k'); first done. lia.
-     + wp_apply (wp_prf_prp_couple_eq_err _ _ _ _ _ _ m2
-                  with "[$Hε $Hg $Hf $HK]"); [done|pose proof(fin_to_nat_lt m2); lia|..].
-       * intros. apply not_elem_of_dom_1. intro.
-         eassert (n' ∈ (set_seq 0 (S val_size))).
-         { eapply elem_of_weaken; exact. }
-         rewrite elem_of_set_seq in H2. lia.
-       * pose proof list_pigeonhole _ _ Hsubseteq as H0.
-         pose proof Nat.lt_ge_cases  (S val_size) (length l) as [H1|H1]; try lia.
-         rewrite fmap_length seq_length in H0.
-         specialize (H0 H1).
-         destruct H0 as (?&?&?&?&?&?).
-         eapply NoDup_lookup in HNoDup; [|exact H2|exact H3].
-         subst. lia.
-       * simpl. rewrite Rdiv_def. f_equal. rewrite minus_INR; last lia.
-         rewrite Rdiv_def. apply Rmult_le_compat_r; first pose proof pos_INR_S val_size as H0.
-         { rewrite -Rdiv_1_l. apply Rcomplements.Rdiv_le_0_compat; try lra. done. }
-         rewrite Rcomplements.Rle_minus_l.
-         trans (INR n - INR (S k') + INR (S val_size - (n - S k')))%R; last first.
-         { apply Rplus_le_compat_l. apply le_INR. lia. }
-         rewrite minus_INR; last lia.
-         assert (0<=INR n - INR (S k') - INR (n-S k'))%R; last first.
-         { replace (match val_size with | _ => _  end) with (INR (S val_size)); last by simpl.
-           lra. }
-         rewrite minus_INR; last lia.
-         lra.
-       * iIntros (z) "(HK & Hf & (%l1 & %l2 & %Hperm & Hg))".
-         do 3 wp_pure.
-         simpl.
-         do 3 tp_pure.
-         assert (#(S k' - 1) = #k') as ->.
-         {
-           do 3 f_equal. lia.
-         }
-         iApply ("IH" with "[][][][][][][][$Hε' $Hf $HK $Hg][HΦ]").
-         -- iPureIntro; lia.
-         -- iPureIntro.
-            apply le_S_n.
-            replace (S (S _ - _)) with (S val_size - (n - S k')) by lia.
-            trans (length l); try done.
-            subst. rewrite !app_length cons_length. lia.
-         -- iPureIntro. subst. apply NoDup_app. apply NoDup_app in HNoDup.
-            destruct HNoDup as [?[? HNoDup]]. apply NoDup_cons in HNoDup. set_solver.
-         -- iPureIntro. rewrite list_subseteq_app_iff_l. split; set_solver.
-         -- iPureIntro. intro. subst. rewrite map_img_insert_notin; last done.
-            rewrite elem_of_union elem_of_app. intros [|] [|]; subst.
-            ++ set_unfold. subst. apply NoDup_app in HNoDup. set_solver.
-            ++ set_unfold. subst. apply NoDup_app in HNoDup.
-               destruct HNoDup as [?[? HNoDup]]. apply NoDup_cons in HNoDup.
-               set_solver.
-            ++ eapply Hdom; set_solver.
-            ++ eapply Hdom; set_solver.
-         -- iPureIntro. intros. subst.
-            rewrite dom_insert_L.
-            apply union_least; last done.
-            rewrite singleton_subseteq_l.
-            rewrite <-set_seq_S_start.
-            rewrite elem_of_set_seq.
-            pose proof (fin_to_nat_lt m2).
-            lia.
-         -- simpl. rewrite Rdiv_def. iPureIntro. repeat f_equal. rewrite fold_symmetric; try (intros; lia).
-            apply Req_le. replace (S _)  with (n-k'); first done. lia.
-         -- iModIntro; done.
-            Unshelve.
-            ++ apply gset_semi_set.
-  Qed.
-
-  Lemma wp_prf_prp_test_err E K (n : nat) (ε : R):
-    (INR (fold_left (Nat.add) (seq 0 n) 0%nat) / INR (S val_size))%R = ε ->
-    {{{ ⤇ fill K (test_prp #n) ∗ ↯ ε }}}
-      test_prf #n @ E
-    {{{ f, RET f;
-        ∃ g m l, ⤇ fill K (of_val g) ∗ is_random_function f m∗
-          is_sprp g m l }}}.
- Proof.
-   iIntros (Hε Φ) "(HK & Herr) HΦ ".
-
-   rewrite /test_prf.
-   wp_pure.
-   wp_bind (random_function _).
-   wp_apply (wp_random_function); first done.
-   iIntros (f) "Hf".
-   do 2 wp_pure.
-
-   rewrite /test_prp.
-   tp_pure.
-   tp_bind (random_permutation _).
-   iMod (spec_random_permutation with "HK") as (g) "(HK & Hg)".
-   iSimpl in "HK".
-   do 5 tp_pure.
-   do 3 wp_pure.
-   wp_apply (wp_prf_prp_test_err_ind with "[$Herr $Hf $HK $Hg]"); [..|done].
-   - split; first lia. done.
-   - simpl. rewrite fmap_length seq_length. lia.
-   - intros. apply NoDup_fmap_2; last apply NoDup_seq. apply Nat2Z.inj'.
-   - intros; set_solver.
-   - set_solver.
-   - set_solver.
-   - replace (_-_) with 0; try lia. rewrite <-Hε. done.
- Qed.
-
-
-End prf_prp.
+End prp_prf.
